Updates

generic/Zeta.Generic.TSLog.fst
@@ -1,9 +1,101 @@
 module Zeta.Generic.TSLog
 
+open Zeta.SSeq
+module T = Zeta.Generic.Thread
+
 (* clock is idxfn_t, so has the prefix property *)
 let lemma_prefix_clock_sorted (#vspec #n:_) (itsl: its_log vspec n) (i:nat{i <= length itsl}):
   Lemma (ensures (clock_sorted (prefix itsl i)))
   = admit()
 
-let create (#vspec:_) (gl: G.verifiable_log vspec): (itsl:its_log vspec (S.length gl){to_glog itsl == gl})
+let lemma_empty_verifiable_clock_sorted (vspec: verifier_spec) (n:_)
+  : Lemma (ensures (let il = empty_interleaving (verifier_log_entry vspec) n in
+                    verifiable il /\ clock_sorted il))
   = admit()
+
+let lemma_empty_interleaving_empty_sseq (vspec: verifier_spec) (n:_)
+  : Lemma (ensures (let il = empty_interleaving (verifier_log_entry vspec) n in
+                    let gl = empty (verifier_log_entry vspec) n in
+                    to_glog il == gl))
+  = admit()
+
+(* a thread with at least one entry *)
+let non_empty_thread
+  (#vspec:_)
+  (gl: G.verifiable_log vspec)
+  (tid: SA.seq_index gl)
+  = S.length (S.index gl tid) > 0
+
+(* return the max clock in a thread - the last log entry in the thread *)
+let max_clock_in_thread
+  (#vspec:_)
+  (gl: G.verifiable_log vspec)
+  (tid: _ {non_empty_thread gl tid})
+  : timestamp
+  = let l = S.index gl tid in
+    let n = S.length l in
+    G.clock gl (tid, n-1)
+
+(* for any index within a thread, the max_clock is indeed max *)
+let lemma_max_clock_in_thread_correct
+  (#vspec:_)
+  (gl: G.verifiable_log vspec)
+  (ti: sseq_index gl)
+  : Lemma (ensures(let t,_ = ti in                        (* thread id*)
+                   let c = G.clock gl ti in               (* clock of entry ti *)
+                   c `ts_leq` max_clock_in_thread gl t))
+  = admit()
+
+(* a thread tid has max clock property if it has the max clock overall *)
+let max_clock_prop (#vspec) (gl: G.verifiable_log vspec) (tid: _)
+  = non_empty_thread gl tid /\
+    (forall tid'.
+      {:pattern (max_clock_in_thread gl tid' `ts_leq` max_clock_in_thread gl tid)}
+    (non_empty_thread gl tid' ==> max_clock_in_thread gl tid' `ts_leq` max_clock_in_thread gl tid))
+
+let find_max_clock_thread (#vspec:_) (gl: G.verifiable_log vspec {flat_length gl > 0})
+  : tid: _ {max_clock_prop gl tid}
+  = admit()
+
+let gl_thread_prefix_verifiable
+  (#vspec:_)
+  (gl: G.verifiable_log vspec)
+  (tid: _ {non_empty_thread gl tid})
+  : Lemma (ensures (G.verifiable (sseq_prefix gl tid)))
+          [SMTPat (sseq_prefix gl tid)]
+  = admit()
+
+let rec create 
+  (#vspec:_) 
+  (gl: G.verifiable_log vspec):
+  Tot (itsl:its_log vspec (S.length gl){to_glog itsl == gl})
+  (decreases (flat_length gl))
+  = let m = flat_length gl in
+    let n = S.length gl in
+    if m = 0 then
+    (
+      (* if gl has flat_length zero, then it is empty *)
+      lemma_flat_length_zero gl;
+      assert(gl == empty _ n);
+
+      (* empty interleaving has the required properties *)
+      let itsl = empty_interleaving (verifier_log_entry vspec) n in
+      lemma_empty_verifiable_clock_sorted vspec n;
+      lemma_empty_interleaving_empty_sseq vspec n;
+      itsl
+    )
+    else
+    (
+      let tid = find_max_clock_thread gl in
+      let tl = G.index gl tid in
+      let tn = T.length tl in
+      //assert(T.clock tl (tn - 1) = max_clock_in_thread gl tid);
+
+      (* get a "prefix" of gl by eliminating the last log entry of thread tid *)
+      let gl' = sseq_prefix gl tid in
+
+      (* recursively construct the interleaving for gl' *)
+      let itsl' = create gl' in
+
+      admit()
+    )
