utils/Zeta.SSeq.fst
@@ -192,3 +192,13 @@ let rec lemma_flat_length_zero (#a:_) (ss: sseq a {flat_length ss = 0})
       FStar.Classical.forall_intro aux;
       assert(equal ss en)
     )
+
+let sseq_prefix (#a:_) (ss: sseq a) (i: seq_index ss{length (index ss i) > 0})
+  : ss': sseq a
+    {
+      length ss' = length ss /\
+      flat_length ss' = flat_length ss - 1 /\
+      index ss' i == hprefix (index ss i) /\
+      (forall i'. i' <> i ==> index ss' i' == index ss i')
+    }
+  = admit()
